bedrock2/src/bedrock2/MetricProgramLogic.v
@@ -4,6 +4,7 @@ Require Import bedrock2.Syntax.
 Require Import bedrock2.MetricWeakestPrecondition.
 Require Import bedrock2.MetricWeakestPreconditionProperties.
 Require Import bedrock2.MetricLoops.
+Require bedrock2.ProgramLogic.
 Require Import bedrock2.Map.SeparationLogic bedrock2.Scalars.
 
 Definition spec_of (procname:String.string) := Semantics.env -> Prop.
@@ -143,50 +144,9 @@ Ltac straightline_cleanup :=
 Import MetricWeakestPrecondition.
 Import coqutil.Map.Interface.
 
-Ltac straightline_stackalloc :=
-  match goal with Hanybytes: Memory.anybytes ?a ?n ?mStack |- _ =>
-  let m := match goal with H : map.split ?mCobined ?m mStack |- _ => m end in
-  let mCombined := match goal with H : map.split ?mCobined ?m mStack |- _ => mCobined end in
-  let Hsplit := match goal with H : map.split ?mCobined ?m mStack |- _ => H end in
-  let Hm := multimatch goal with H : _ m |- _ => H end in
-  let Hm' := fresh Hm in
-  let Htmp := fresh in
-  let Pm := match type of Hm with ?P m => P end in
-  assert_fails (assert (Separation.sep Pm (Array.array Separation.ptsto (Interface.word.of_Z (BinNums.Zpos BinNums.xH)) a _) mCombined) as _ by ecancel_assumption);
-  rename Hm into Hm';
-  let stack := fresh "stack" in
-  let stack_length := fresh "length_" stack in (* MUST remain in context for deallocation *)
-  destruct (Array.anybytes_to_array_1 mStack a n Hanybytes) as (stack&Htmp&stack_length);
-  epose proof (ex_intro _ m (ex_intro _ mStack (conj Hsplit (conj Hm' Htmp)))
-  : Separation.sep _ (Array.array Separation.ptsto (Interface.word.of_Z (BinNums.Zpos BinNums.xH)) a _) mCombined) as Hm;
-  clear Htmp; (* note: we could clear more here if we assumed only one separation-logic description of each memory is present *)
-  try (let m' := fresh m in rename m into m'); rename mCombined into m;
-  ( assert (BinInt.Z.of_nat (Datatypes.length stack) = n)
-  by (rewrite stack_length; apply (ZifyInst.of_nat_to_nat_eq n))
-  || fail 2 "negative stackalloc of size" n )
-  end.
+Ltac straightline_stackalloc := ProgramLogic.straightline_stackalloc.
 
-Ltac straightline_stackdealloc :=
-  lazymatch goal with |- exists _ _, Memory.anybytes ?a ?n _ /\ map.split ?m _ _ /\ _ =>
-  let Hm := multimatch goal with Hm : _ m |- _ => Hm end in
-  let stack := match type of Hm with context [Array.array Separation.ptsto _ a ?stack] => stack end in
-  let length_stack := match goal with H : Datatypes.length stack = _ |- _ => H end in
-  let Hm' := fresh Hm in
-  pose proof Hm as Hm';
-  let Psep := match type of Hm with ?P _ => P end in
-  let Htmp := fresh "Htmp" in
-  eassert (Lift1Prop.iff1 Psep (Separation.sep _ (Array.array Separation.ptsto (Interface.word.of_Z (BinNums.Zpos BinNums.xH)) a stack))) as Htmp
-  by ecancel || fail "failed to find stack frame in" Psep "using ecancel";
-  eapply (fun m => proj1 (Htmp m)) in Hm;
-  let m' := fresh m in
-  rename m into m';
-  let mStack := fresh in
-  destruct Hm as (m&mStack&Hsplit&Hm&Harray1); move Hm at bottom;
-  pose proof Array.array_1_to_anybytes _ _ _ Harray1 as Hanybytes;
-  rewrite length_stack in Hanybytes;
-  refine (ex_intro _ m (ex_intro _ mStack (conj Hanybytes (conj Hsplit _))));
-  clear Htmp Hsplit mStack Harray1 Hanybytes
-  end.
+Ltac straightline_stackdealloc := ProgramLogic.straightline_stackdealloc.
 
 Ltac rename_to_different H :=
   idtac;
