bedrock2/src/bedrock2/MetricSemantics.v
@@ -101,14 +101,14 @@ Module exec. Section WithParams.
   | stackalloc x n body
     t mSmall l mc post
     (_ : Z.modulo n (bytes_per_word width) = 0)
-    (_ : forall a mStack mCombined,
-        anybytes a n mStack ->
-        map.split mCombined mSmall mStack ->
+    (_ : forall a stack mCombined,
+        Z.of_nat (length stack) = n ->
+        map.split mCombined mSmall (map.of_list_word_at a stack) ->
         exec body t mCombined (map.put l x a) (cost_stackalloc isRegStr x mc)
           (fun t' mCombined' l' mc' =>
-            exists mSmall' mStack',
-              anybytes a n mStack' /\
-              map.split mCombined' mSmall' mStack' /\
+            exists mSmall' (stack' : list byte),
+              map.split mCombined' mSmall' (map.of_list_word_at a stack') /\
+              Z.of_nat (length stack') = n /\
               post t' mSmall' l' mc'))
      : exec (cmd.stackalloc x n body) t mSmall l mc post
   | if_true t m l mc e c1 c2 post
@@ -231,7 +231,10 @@ Module exec. Section WithParams.
         specialize @map.split_diff with (4 := A) (5 := B) as P
       end.
       edestruct P; try typeclasses eauto. 2: subst; eauto 10.
-      eapply anybytes_unique_domain; eassumption.
+      { (* same_domain_of_list_word_at *)
+        cbv [map.same_domain map.sub_domain]; setoid_rewrite map.get_of_list_word_at.
+        split; intros ? ? ?%List.nth_error_Some_bound_index;
+        eexists; unshelve eapply List.nth_error_nth'; try Lia.lia; try constructor. }
     - econstructor.
       + eapply IHexec. exact H5. (* not H *)
       + simpl. intros *. intros [? ?]. eauto.
